correct a dependency order problem that dafny misses if you don't verify every file

chapter06/exercises/distributed_system.s.dfy
@@ -10,22 +10,6 @@ include "protocol.i.dfy"
 // Before we get here, caller must define a type Message that we'll
 // use to instantiate network.s.dfy.
 
-// A global constant telling us how many hosts are participating.  It's a
-// constant so we don't have to prove it doesn't change as the execution
-// evolves.
-function NumHosts() : nat
-  ensures NumHosts() > 0
-
-// "newtype" means that HostId is just an int ... except that it always
-// satisfies 0 <= b < NumHosts().
-// ("nat" is "newtype nat = b: int | 0 <= b".)
-newtype HostId = b: int | 0 <= b < NumHosts()
-
-// The set of all host identities.
-function AllHosts() : set<HostId> {
-  set h:HostId | true     // ignore the "No terms found" warning.
-}
-
 datatype DistState = DistState(
   hosts:map<HostId, HostState>, network:NetState<Message>)
 
